theories/iris_fundamental_call_indirect.v
@@ -27,10 +27,10 @@ Section fundamental.
       ∃ τt a, ⌜(tc_table C) !! 0 = Some τt⌝
             ∗ ⌜(inst_tab j) !! 0 = Some a⌝
             ∗ ∃ table_size, (N.of_nat a) ↪[wtsize] table_size
-                          ∗ (interp_table (HWP:=HWP) table_size) j (interp_instance (HWP:=HWP) C) (N.of_nat a).
+                          ∗ (interp_table (HWP:=HWP) table_size) (N.of_nat a).
   Proof.
     iIntros (Hnil) "#Hi".
-    destruct C,j. rewrite fixpoint_interp_instance_eq /=.
+    destruct C,j.
     iDestruct "Hi" as "[_ [_ [Hi _]]]". simpl in Hnil.
     destruct (nth_error tc_table 0) eqn:Ht0;cycle 1.
     { exfalso. rewrite nth_error_lookup in Ht0.
@@ -48,7 +48,7 @@ Section fundamental.
       ⌜nth_error (inst_types j) i = Some tf⌝.
   Proof.
     iIntros (Hnth) "#Hi".
-    destruct C,j. rewrite fixpoint_interp_instance_eq /=. simpl in *.
+    destruct C,j.
     iDestruct "Hi" as "[%Heq _]".
     rewrite Heq. auto.
   Qed.
@@ -194,22 +194,12 @@ Section fundamental.
         iApply wp_wasm_empty_ctx_frame.
         take_drop_app_rewrite 0.
         iApply (wp_block_local_ctx with "Hf");eauto.
-        destruct (instance_eq_dec i0 j).
-        
-        { iNext. iIntros "Hf".
-          iApply wp_label_push_nil_local. simpl push_base.
-          unfold interp_closure_native.
-          erewrite app_nil_l.
-          rewrite e0. iDestruct ("Hcl" with "Hi") as "Hcl'".
-          iApply ("Hcl'" with "[] Hown Hf").
-          iRight. iExists _. eauto. }
-
-        { iNext. iIntros "Hf".
-          iApply wp_label_push_nil_local. simpl push_base.
-          unfold interp_closure_native.
-          erewrite app_nil_l.
-          iApply ("Hcl" with "[] Hown Hf").
-          iRight. iExists _. eauto. }
+        iNext. iIntros "Hf".
+        iApply wp_label_push_nil_local. simpl push_base.
+        unfold interp_closure_native.
+        erewrite app_nil_l.
+        iApply ("Hcl" with "[] Hown Hf").
+        iRight. iExists _. eauto.
       }
       { (* host function *)
         destruct f.
